[TODO: DROP] Gordon's wordLang

compiler/backend/semantics/wordSemScript.sml
@@ -94,6 +94,7 @@ val _ = Datatype `
      ; stack_size : num num_map (* stack frame size of function, unbounded if unmapped *)
      ; memory  : 'a word -> 'a word_loc
      ; mdomain : ('a word) set
+     ; sh_mdomain : ('a word) set
      ; permute : num -> num -> num (* sequence of bijective mappings *)
      ; compile : 'c -> (num # num # 'a wordLang$prog) list -> (word8 list # 'a word list # 'c) option
      ; compile_oracle : num -> 'c # (num # num # 'a wordLang$prog) list
@@ -225,6 +226,74 @@ val flush_state_def = Define `
                               ; locals_size := SOME 0 |>
 /\ flush_state F ^s = s with <| locals := LN
                               ; locals_size := SOME 0 |>`;
+
+(* clean up *)
+(* length, 'a word, endianness *)
+(* cyclic repeat as get_byte does when length > 'a bytes_in_word *)
+Definition word_to_bytes_aux_def:
+  word_to_bytes_aux 0 (w:'a word) be = [] ∧
+  word_to_bytes_aux (SUC n) w be =
+    (word_to_bytes_aux n w be) ++ [get_byte (n2w n) w be]
+End
+
+Definition word_to_bytes_def:
+  word_to_bytes (w:'a word) be =
+  word_to_bytes_aux (dimindex (:'a) DIV 8) w be
+End
+
+Definition sh_mem_store_def:
+  sh_mem_store (a:'a word) (w:'a word) ^s =
+    if a IN s.sh_mdomain then
+      case call_FFI s.ffi "MappedWrite" [0w:word8]
+                    (word_to_bytes w F ++ word_to_bytes a F) of
+      | FFI_final outcome => (SOME (FinalFFI outcome), flush_state T s)
+      | FFI_return new_ffi new_bytes => (NONE, (s with ffi := new_ffi))
+    else (SOME Error, s)
+End
+
+Definition sh_mem_load_def:
+  sh_mem_load (a:'a word) ^s =
+    if a IN s.sh_mdomain then
+      SOME $ call_FFI s.ffi "MappedRead" [0w:word8]
+                    (word_to_bytes a F)
+    else NONE
+End
+
+Definition sh_mem_store_byte_def:
+  sh_mem_store_byte (a:'a word) (w:'a word) ^s =
+    if byte_align a IN s.sh_mdomain then
+      case call_FFI s.ffi "MappedWrite" [1w:word8]
+                    ([get_byte 0w w F] ++ word_to_bytes a F) of
+        FFI_final outcome => (SOME (FinalFFI outcome), flush_state T s)
+      | FFI_return new_ffi new_bytes => (NONE, (s with ffi := new_ffi))
+    else (SOME Error, s)
+End
+
+Definition sh_mem_load_byte_def:
+  sh_mem_load_byte (a:'a word) ^s =
+    if byte_align a IN s.sh_mdomain then
+      SOME $ call_FFI s.ffi "MappedRead" [1w:word8]
+                    (word_to_bytes a F)
+    else NONE
+End
+
+(* set variable given the output from ShareLoad(Byte) *)
+Definition sh_mem_set_var_def:
+  (sh_mem_set_var (SOME (FFI_final outcome)) _ ^s = (SOME (FinalFFI outcome), flush_state T s)) /\
+  (sh_mem_set_var (SOME (FFI_return new_ffi new_bytes)) v s = (NONE, set_var v (Word (word_of_bytes F 0w new_bytes)) (s with ffi := new_ffi))) /\
+  (sh_mem_set_var _ _ s = (SOME Error, s))
+End
+
+Definition share_inst_def:
+  (share_inst Load v ad s = sh_mem_set_var (sh_mem_load ad s) v s) /\
+  (share_inst Load8 v ad s = sh_mem_set_var (sh_mem_load_byte ad s) v s) /\
+  (share_inst Store v ad s = case get_var v s of
+    | SOME (Word v) => sh_mem_store ad v s
+    | _ => (SOME Error,s)) /\
+  (share_inst Store8 v ad s = case get_var v s of
+    | SOME (Word v) => sh_mem_store_byte ad v s
+    | _ => (SOME Error,s))
+End
 
 val call_env_def = Define `
   call_env args size ^s =
@@ -815,25 +884,30 @@ val evaluate_def = tDefine "evaluate" `
             (NONE,s with data_buffer:=new_db)
           | _ => (SOME Error,s))
         | _ => (SOME Error,s))) /\
-  (evaluate (FFI ffi_index ptr1 len1 ptr2 len2 names,s) =
-    case (get_var len1 s, get_var ptr1 s, get_var len2 s, get_var ptr2 s) of
-    | SOME (Word w),SOME (Word w2),SOME (Word w3),SOME (Word w4) =>
-      (case cut_env names s.locals of
-      | NONE => (SOME Error,s)
-      | SOME env =>
-        (case (read_bytearray w2 (w2n w) (mem_load_byte_aux s.memory s.mdomain s.be),
-               read_bytearray w4 (w2n w3) (mem_load_byte_aux s.memory s.mdomain s.be))
-               of
-          | SOME bytes,SOME bytes2 =>
-             (case call_FFI s.ffi ffi_index bytes bytes2 of
-              | FFI_final outcome => (SOME (FinalFFI outcome),flush_state T s)
-              | FFI_return new_ffi new_bytes =>
-                let new_m = write_bytearray w4 new_bytes s.memory s.mdomain s.be in
-                  (NONE, s with <| memory := new_m ;
-                                   locals := env ;
-                                   ffi := new_ffi |>))
-          | _ => (SOME Error,s)))
-    | res => (SOME Error,s)) /\
+  (evaluate (FFI ffi_index ptr1 len1 ptr2 len2 names,s) =  if ffi_index <> "MappedRead" /\ ffi_index <> "MappedWrite" then
+      (case (get_var len1 s, get_var ptr1 s, get_var len2 s, get_var ptr2 s) of
+      | SOME (Word w),SOME (Word w2),SOME (Word w3),SOME (Word w4) =>
+        (case cut_env names s.locals of
+        | NONE => (SOME Error,s)
+        | SOME env =>
+          (case (read_bytearray w2 (w2n w) (mem_load_byte_aux s.memory s.mdomain s.be),
+                 read_bytearray w4 (w2n w3) (mem_load_byte_aux s.memory s.mdomain s.be))
+                 of
+            | SOME bytes,SOME bytes2 =>
+               (case call_FFI s.ffi ffi_index bytes bytes2 of
+                | FFI_final outcome => (SOME (FinalFFI outcome),flush_state T s)
+                | FFI_return new_ffi new_bytes =>
+                  let new_m = write_bytearray w4 new_bytes s.memory s.mdomain s.be in
+                    (NONE, s with <| memory := new_m ;
+                                     locals := env ;
+                                     ffi := new_ffi |>))
+            | _ => (SOME Error,s)))
+      | res => (SOME Error,s))
+    else (SOME Error,s)) /\
+  (evaluate (ShareInst op v exp, s) =
+    (case word_exp s exp of
+    | SOME (Word ad) => share_inst op v ad s
+    | _ => (SOME Error,s))) /\
   (evaluate (Call ret dest args handler,s) =
     case get_vars args s of
     | NONE => (SOME Error,s)
@@ -927,6 +1001,30 @@ Proof
   \\ rpt var_eq_tac \\ full_simp_tac(srw_ss())[]
 QED
 
+Theorem sh_mem_set_var_clock:
+  !v s1 v2 s2 res.
+    (sh_mem_set_var res v s1 = (v2,s2)) ==>
+    s2.clock <= s1.clock /\ s2.termdep = s1.termdep
+Proof
+  Cases_on `res` >>
+  simp[sh_mem_set_var_def] >>
+  Cases_on `x` >>
+  simp[sh_mem_set_var_def,set_var_def,flush_state_def]
+QED
+
+Theorem share_inst_clock:
+  !op v ad s1 v1 s2.
+    (share_inst op v ad s1 = (v2, s2)) ==>
+    s2.clock <= s1.clock /\ s2.termdep = s1.termdep
+Proof
+  Cases_on `op` >>
+  simp[share_inst_def] >>
+  rpt strip_tac >>
+  gvs[AllCaseEqs(),sh_mem_store_def,sh_mem_store_byte_def,flush_state_def] >>
+  drule sh_mem_set_var_clock >>
+  simp[]
+QED
+
 val inst_clock = Q.prove(
   `inst i s = SOME s2 ==> s2.clock <= s.clock /\ s2.termdep = s.termdep`,
   Cases_on `i` \\ full_simp_tac(srw_ss())[inst_def,assign_def,get_vars_def,LET_THM]
@@ -950,7 +1048,8 @@ Proof
   \\ rpt var_eq_tac \\ full_simp_tac(srw_ss())[]
   \\ full_simp_tac(srw_ss())[set_vars_def,set_var_def,set_store_def,unset_var_def]
   \\ imp_res_tac inst_clock \\ full_simp_tac(srw_ss())[]
-  \\ full_simp_tac(srw_ss())[mem_store_def,call_env_def,dec_clock_def,flush_state_def]
+  \\ imp_res_tac share_inst_clock
+  \\ fs[mem_store_def,call_env_def,dec_clock_def,flush_state_def]
   \\ rpt var_eq_tac \\ full_simp_tac(srw_ss())[]
   \\ full_simp_tac(srw_ss())[LET_THM] \\ rpt (pairarg_tac \\ full_simp_tac(srw_ss())[])
   \\ full_simp_tac(srw_ss())[jump_exc_def,pop_env_def]
@@ -963,7 +1062,7 @@ Proof
   \\ TRY (PairCases_on `x''`)
   \\ full_simp_tac(srw_ss())[push_env_def,LET_THM]
   \\ rpt (pairarg_tac \\ full_simp_tac(srw_ss())[])
-  \\ decide_tac
+  \\ TRY decide_tac
 QED
 
 Theorem fix_clock_evaluate[local]:
@@ -1015,20 +1114,6 @@ Definition word_lang_safe_for_space_def:
     let prog = Call NONE (SOME start) [0] NONE in
       (!k res t. wordSem$evaluate (prog, s with clock := k) = (res,t) ==>
         ?max. t.stack_max = SOME max /\ max <= t.stack_limit)
-End
-
-(* clean up *)
-(* length, 'a word, endianness *)
-(* cyclic repeat as get_byte does when length > 'a bytes_in_word *)
-Definition word_to_bytes_aux_def:
-  word_to_bytes_aux 0 (w:'a word) be = [] ∧
-  word_to_bytes_aux (SUC n) w be =
-    (word_to_bytes_aux n w be) ++ [get_byte (n2w n) w be]
-End
-
-Definition word_to_bytes_def:
-  word_to_bytes (w:'a word) be =
-  word_to_bytes_aux (dimindex (:'a) DIV 8) w be
 End
 
 val _ = map delete_binding ["evaluate_AUX_def", "evaluate_primitive_def"];
